simulate: use immediate for local alloc

CoqOfRust/revm/revm_interpreter/instructions/simulate/arithmetic.v
@@ -3,181 +3,13 @@ Require Import CoqOfRust.links.M.
 Require Import CoqOfRust.simulate.M.
 Require Import alloy_primitives.links.aliases.
 Require Import revm.revm_context_interface.links.host.
+Require Import revm.revm_interpreter.gas.simulate.constants.
 Require Import revm.revm_interpreter.instructions.links.arithmetic.
 Require Import revm.revm_interpreter.links.gas.
 Require Import revm.revm_interpreter.links.interpreter.
 Require Import revm.revm_interpreter.links.interpreter_types.
-
-Definition make_ref {A : Set} `{Link A} {kind : Pointer.Kind.t} (index : nat) : Ref.t kind A :=
-  {| Ref.core := Ref.Core.Mutable (A := A) index [] φ Some (fun _ => Some) |}.
-
-Module RefStub.
-  Record t {A Sub_A : Set} `{Link A} `{Link Sub_A} : Set := {
-    path : Pointer.Path.t;
-    (* We suppose the pointer is valid (no [option] type for the [projection] and [injection]
-       functions) *)
-    projection : A -> Sub_A;
-    injection : A -> Sub_A -> A;
-  }.
-  Arguments t _ _ {_ _}.
-
-  Definition apply_core {A Sub_A : Set} `{Link A} `{Link Sub_A}
-      (ref_core : Ref.Core.t A)
-      (stub : t A Sub_A) :
-      Ref.Core.t Sub_A.
-  Proof.
-    destruct ref_core as [| ? ? address path big_to_value projection injection].
-    { (* Immediate *)
-      exact (
-        Ref.Core.Immediate (
-          match value with
-          | Some a => Some (stub.(projection) a)
-          | None => None
-          end
-        )
-      ).
-    }
-    { (* Mutable *)
-      exact (
-        Ref.Core.Mutable
-          address
-          (path ++ stub.(RefStub.path))
-          big_to_value
-          (fun big_a =>
-            match projection big_a with
-            | Some a => Some (stub.(RefStub.projection) a)
-            | None => None
-            end
-          )
-          (fun big_a new_sub_a =>
-            match projection big_a with
-            | Some a =>
-              let new_a := stub.(RefStub.injection) a new_sub_a in
-              injection big_a new_a
-            | None => None
-            end
-          )
-      ).
-    }
-  Defined.
-
-  Definition apply {A Sub_A : Set} `{Link A} `{Link Sub_A}
-      {kind_source kind_target : Pointer.Kind.t}
-      (ref : Ref.t kind_source A)
-      (stub : t A Sub_A) :
-      Ref.t kind_target Sub_A :=
-    {| Ref.core := apply_core ref.(Ref.core) stub |}.
-End RefStub.
-
-Module Loop.
- Class C
-      (WIRE_types : InterpreterTypes.Types.t) `{InterpreterTypes.Types.AreLinks WIRE_types} :
-      Set := {
-    gas : RefStub.t WIRE_types.(InterpreterTypes.Types.Control) Gas.t;
-  }.
-
-  Module Eq.
-    Class t
-        (WIRE : Set) (WIRE_types : InterpreterTypes.Types.t)
-        `{Link WIRE} `{InterpreterTypes.Types.AreLinks WIRE_types}
-        (run_InterpreterTypes_for_WIRE : InterpreterTypes.Run WIRE WIRE_types)
-        (I : C WIRE_types) :
-        Prop := {
-      gas
-          (Stack : list Set)
-          (interpreter : Interpreter.t WIRE WIRE_types)
-          (stack_rest : Stack.to_Set Stack) :
-        let ref_interpreter : Ref.t Pointer.Kind.MutRef _ := make_ref 0 in
-        let ref_self := {| Ref.core :=
-            SubPointer.Runner.apply
-              ref_interpreter.(Ref.core)
-              Interpreter.SubPointer.get_control
-        |} in
-        {{
-          StackM.eval_f (Stack := Interpreter.t WIRE WIRE_types :: Stack)
-            (run_InterpreterTypes_for_WIRE.(InterpreterTypes.run_LoopControl_for_Control).(LoopControl.gas).(TraitMethod.run)
-              ref_self
-            )
-            (interpreter, stack_rest) 🌲
-          (Output.Success (RefStub.apply ref_self I.(gas)), (interpreter, stack_rest))
-        }};
-    }.
-  End Eq.
-End Loop.
-
-Module Stack.
-  (* Definition t : Set :=
-    list aliases.U256.t. *)
-
-  (* Fixpoint popn_top (POPN : nat) (stack : t) :
-      option (array.t aliases.U256.t {| Integer.value := Z.of_nat POPN |}) * t :=
-    match POPN, stack with
-    | O, [] => (Some {| array.value := [] |}, stack)
-    | S POPN, [] => (None, stack)
-    | S POPN, x :: xs =>
-        match popn_top POPN xs with
-        | (Some a, stack') => (Some {| array.value := x:: a.(array.value) |}, stack')
-        | (None, _) => (None, stack)
-        end
-    | _, _ => (None, stack)
-    end. *)
-
-  (* Definition pop2_top (stack : t) : option (array.t aliases.U256.t {| Integer.value := 2 |}) * t :=
-    match stack with
-    | x1 :: x2 :: rest => (Some {| array.value := [x1; x2] |}, rest)
-    | _ => (None, stack)
-    end. *)
-
-  Class C
-      (WIRE_types : InterpreterTypes.Types.t) `{InterpreterTypes.Types.AreLinks WIRE_types} :
-      Type := {
-    popn_top :
-      forall
-        (POPN : Usize.t)
-        (self : WIRE_types.(InterpreterTypes.Types.Stack)),
-      option (
-        array.t aliases.U256.t POPN *
-        RefStub.t WIRE_types.(InterpreterTypes.Types.Stack) aliases.U256.t
-      ) *
-      WIRE_types.(InterpreterTypes.Types.Stack);
-  }.
-
-  Module Eq.
-    Class t
-        (WIRE : Set) (WIRE_types : InterpreterTypes.Types.t)
-        `{Link WIRE} `{InterpreterTypes.Types.AreLinks WIRE_types}
-        (run_InterpreterTypes_for_WIRE : InterpreterTypes.Run WIRE WIRE_types)
-        (I : C WIRE_types) :
-        Prop := {
-      popn_top
-          (Stack : list Set)
-          (interpreter : Interpreter.t WIRE WIRE_types)
-          (stack_rest : Stack.to_Set Stack)
-          (POPN : Usize.t) :
-        let ref_interpreter : Ref.t Pointer.Kind.MutRef _ := make_ref 0 in
-        let ref_self := {| Ref.core :=
-          SubPointer.Runner.apply
-            ref_interpreter.(Ref.core)
-            Interpreter.SubPointer.get_stack
-        |} in
-        {{
-          StackM.eval_f (Stack := Interpreter.t WIRE WIRE_types :: Stack)
-            (run_InterpreterTypes_for_WIRE.(InterpreterTypes.run_StackTrait_for_Stack).(StackTrait.popn_top).(TraitMethod.run)
-              POPN
-              ref_self
-            )
-            (interpreter, stack_rest) 🌲
-          let (result, self) := I.(popn_top) POPN interpreter.(Interpreter.stack) in
-          let result :=
-            match result with
-            | Some (a, stub) => Some (a, RefStub.apply ref_self stub)
-            | None => None
-            end in
-          (Output.Success result, (interpreter <| Interpreter.stack := self |>, stack_rest))
-        }};
-    }.
-  End Eq.
-End Stack.
+Require Import revm.revm_interpreter.simulate.gas.
+Require Import revm.revm_interpreter.simulate.interpreter_types.
 
 Parameter wrapping_add :
   forall {BITS LIMBS : Usize.t} (x1 x2 : lib.Uint.t BITS LIMBS),
@@ -228,45 +60,35 @@ Lemma add_eq
 Proof.
   intros.
   destruct LoopEq, StackEq.
-  Time unfold run_add, StackM.eval_f, StackM.eval, evaluate.
-  Time hnf.
-  Time cbn.
-  Time get_can_access.
-  Time cbn.
-  Time eapply Run.Call. {
+  unfold run_add, StackM.eval_f, StackM.eval, evaluate.
+  eapply Run.Call. {
     apply gas.
   }
-  Time cbn.
-  Time eapply Run.Call. {
-    Time apply Run.Pure.
+  eapply Run.Call. {
+    apply VERYLOW_eq.
   }
-  Time cbn.
-  Time get_can_access.
-  Show.
-  dsfjlkj.
+  eapply Run.Call. {
+    pose proof (Impl_Gas.record_cost_eq (StackRest := [H]) interpreter) as H_record_cost.
+    apply H_record_cost.
+  }
+  eapply Run.Call. {
+    apply Run.Pure.
+  }
+  eapply Run.Call. {
     apply popn_top.
   }
-  Time destruct IStack.(Stack.popn_top) as [[[? ?]|] ?].
-  { Time get_can_access.
-    Time cbn.
-    Time destruct t0.(array.value).
-    { Time cbn.
-      destruct ex_falso.
-    }
-    { Time cbn.
-      Time repeat get_can_access.
-      Time eapply Run.Call. {
+  destruct IStack.(Stack.popn_top) as [[[? ?]|] ?].
+  { destruct t0 as [t0].
+    destruct t0.
+    { destruct ex_falso. }
+    { progress repeat get_can_access.
+      eapply Run.Call. {
         rewrite wrapping_add_eq.
         apply Run.Pure.
       }
-      Time cbn.
-      (* admit. because slow *)
-      Time repeat get_can_access.
-      Time apply Run.Pure.
+      progress repeat get_can_access.
+      apply Run.Pure.
     }
   }
-  { Time cbn.
-    Time repeat get_can_access.
-    Time apply Run.Pure.
-  }
+  { apply Run.Pure. }
 Qed.
