CoqOfRust/revm/revm_interpreter/gas/simulate/constants.v
@@ -1,0 +1,15 @@
+Require Import CoqOfRust.CoqOfRust.
+Require Import CoqOfRust.links.M.
+Require Import CoqOfRust.simulate.M.
+Require Import revm.revm_interpreter.gas.links.constants.
+
+Lemma VERYLOW_eq {Stack : Stack.t} (stack : Stack.to_Set Stack) :
+  {{
+    StackM.eval_f (Stack := Stack) run_VERYLOW stack 🌲
+    (Output.Success (Ref.immediate _ {| Integer.value := 3 |}), stack)
+  }}.
+Proof.
+  cbn.
+  apply Run.Pure.
+Qed.
+Global Opaque run_VERYLOW.
