CoqOfRust/revm/revm_interpreter/simulate/interpreter_types.v
@@ -1,0 +1,117 @@
+Require Import CoqOfRust.CoqOfRust.
+Require Import CoqOfRust.links.M.
+Require Import CoqOfRust.simulate.M.
+Require Import alloy_primitives.links.aliases.
+Require Import revm.revm_interpreter.links.gas.
+Require Import revm.revm_interpreter.links.interpreter.
+Require Import revm.revm_interpreter.links.interpreter_types.
+
+Module Loop.
+ Class C
+      (WIRE_types : InterpreterTypes.Types.t) `{InterpreterTypes.Types.AreLinks WIRE_types} :
+      Set := {
+    gas : RefStub.t WIRE_types.(InterpreterTypes.Types.Control) Gas.t;
+  }.
+
+  Module Eq.
+    Class t
+        (WIRE : Set) (WIRE_types : InterpreterTypes.Types.t)
+        `{Link WIRE} `{InterpreterTypes.Types.AreLinks WIRE_types}
+        (run_InterpreterTypes_for_WIRE : InterpreterTypes.Run WIRE WIRE_types)
+        (I : C WIRE_types) :
+        Prop := {
+      gas
+          (Stack : list Set)
+          (interpreter : Interpreter.t WIRE WIRE_types)
+          (stack_rest : Stack.to_Set Stack) :
+        let ref_interpreter : Ref.t Pointer.Kind.MutRef _ := make_ref 0 in
+        let ref_self := {| Ref.core :=
+            SubPointer.Runner.apply
+              ref_interpreter.(Ref.core)
+              Interpreter.SubPointer.get_control
+        |} in
+        {{
+          StackM.eval_f (Stack := Interpreter.t WIRE WIRE_types :: Stack)
+            (run_InterpreterTypes_for_WIRE.(InterpreterTypes.run_LoopControl_for_Control).(LoopControl.gas).(TraitMethod.run)
+              ref_self
+            )
+            (interpreter, stack_rest) 🌲
+          (Output.Success (RefStub.apply ref_self I.(gas)), (interpreter, stack_rest))
+        }};
+    }.
+  End Eq.
+End Loop.
+
+Module Stack.
+  (* Definition t : Set :=
+    list aliases.U256.t. *)
+
+  (* Fixpoint popn_top (POPN : nat) (stack : t) :
+      option (array.t aliases.U256.t {| Integer.value := Z.of_nat POPN |}) * t :=
+    match POPN, stack with
+    | O, [] => (Some {| array.value := [] |}, stack)
+    | S POPN, [] => (None, stack)
+    | S POPN, x :: xs =>
+        match popn_top POPN xs with
+        | (Some a, stack') => (Some {| array.value := x:: a.(array.value) |}, stack')
+        | (None, _) => (None, stack)
+        end
+    | _, _ => (None, stack)
+    end. *)
+
+  (* Definition pop2_top (stack : t) : option (array.t aliases.U256.t {| Integer.value := 2 |}) * t :=
+    match stack with
+    | x1 :: x2 :: rest => (Some {| array.value := [x1; x2] |}, rest)
+    | _ => (None, stack)
+    end. *)
+
+  Class C
+      (WIRE_types : InterpreterTypes.Types.t) `{InterpreterTypes.Types.AreLinks WIRE_types} :
+      Type := {
+    popn_top :
+      forall
+        (POPN : Usize.t)
+        (self : WIRE_types.(InterpreterTypes.Types.Stack)),
+      option (
+        array.t aliases.U256.t POPN *
+        RefStub.t WIRE_types.(InterpreterTypes.Types.Stack) aliases.U256.t
+      ) *
+      WIRE_types.(InterpreterTypes.Types.Stack);
+  }.
+
+  Module Eq.
+    Class t
+        (WIRE : Set) (WIRE_types : InterpreterTypes.Types.t)
+        `{Link WIRE} `{InterpreterTypes.Types.AreLinks WIRE_types}
+        (run_InterpreterTypes_for_WIRE : InterpreterTypes.Run WIRE WIRE_types)
+        (I : C WIRE_types) :
+        Prop := {
+      popn_top
+          (Stack : list Set)
+          (interpreter : Interpreter.t WIRE WIRE_types)
+          (stack_rest : Stack.to_Set Stack)
+          (POPN : Usize.t) :
+        let ref_interpreter : Ref.t Pointer.Kind.MutRef _ := make_ref 0 in
+        let ref_self := {| Ref.core :=
+          SubPointer.Runner.apply
+            ref_interpreter.(Ref.core)
+            Interpreter.SubPointer.get_stack
+        |} in
+        {{
+          StackM.eval_f (Stack := Interpreter.t WIRE WIRE_types :: Stack)
+            (run_InterpreterTypes_for_WIRE.(InterpreterTypes.run_StackTrait_for_Stack).(StackTrait.popn_top).(TraitMethod.run)
+              POPN
+              ref_self
+            )
+            (interpreter, stack_rest) 🌲
+          let (result, self) := I.(popn_top) POPN interpreter.(Interpreter.stack) in
+          let result :=
+            match result with
+            | Some (a, stub) => Some (a, RefStub.apply ref_self stub)
+            | None => None
+            end in
+          (Output.Success result, (interpreter <| Interpreter.stack := self |>, stack_rest))
+        }};
+    }.
+  End Eq.
+End Stack.
